theories/lang/cpp/logic/heap_pred/any.v
@@ -1,0 +1,349 @@
+(*
+ * Copyright (c) 2023 BedRock Systems, Inc.
+ * This software is distributed under the terms of the BedRock Open-Source License.
+ * See the LICENSE-BedRock file in the repository root for details.
+ *)
+Require Import bedrock.lang.cpp.logic.heap_pred.prelude.
+From bedrock.lang.cpp.logic.heap_pred Require Import
+  valid everywhere tptsto prim uninit null.
+
+#[local] Set Printing Coercions.
+Implicit Types (σ : genv) (p : ptr) (o : offset).
+
+#[local]
+Definition primitiveR `{Σ : cpp_logic} {σ : genv} q ty :=
+  Exists v,
+    let rty :=
+      match erase_qualifiers ty with
+      | Trv_ref t => Tref t
+      | t => t
+      end
+    in tptstoR rty q v.
+
+(** [anyR] The argument pointers points to a value of C++ type [ty] that might be
+    uninitialized.
+ *)
+mlock
+Definition anyR `{Σ : cpp_logic} {σ : genv} (ty : type) (q : cQp.t) : Rep :=
+  everywhereR σ.(genv_tu) primitiveR q ty.
+#[global] Arguments anyR {_ Σ σ} _ _ : assert.
+
+Section with_cpp.
+  Context `{Σ : cpp_logic} {σ : genv}.
+
+  #[global] Instance anyR_timeless : ∀ ty q, Timeless (anyR ty q).
+  Proof.
+    intros. red.
+    rewrite anyR.unlock.
+    iIntros "X".
+    iDestruct "X" as (f) "X".
+    iExists f.
+    iStopProof.
+    eapply everywhereR_f_timeless. refine _.
+  Qed.
+
+  #[global] Instance anyR_cfractional : ∀ ty, CFractional (anyR ty).
+  Proof.
+    do 3 intro.
+    rewrite anyR.unlock.
+    iSplit.
+    { iIntros "X"; iDestruct "X" as (f) "X".
+      rewrite everywhereR_f_cfractional.
+      iDestruct "X" as "[A B]".
+      iSplitL "A"; iExists _; iFrame. }
+    { iIntros "[A B]".
+      iDestruct "A" as (fa) "A".
+      iDestruct "B" as (fb) "B".
+      iExists (max fa fb).
+      rewrite everywhereR_f_cfractional.
+      iSplitL "A".
+      - rewrite -(_offsetR_id (everywhereR_f _ _ fa _ _)).
+        rewrite -(_offsetR_id (everywhereR_f _ _ (_ `max` _) _ _)).
+        iRevert "A".
+        iApply everywhereR_f_mono'. lia.
+      - rewrite -(_offsetR_id (everywhereR_f _ _ fb _ _)).
+        rewrite -(_offsetR_id (everywhereR_f _ _ (_ `max` _) _ _)).
+        iRevert "B".
+        iApply everywhereR_f_mono'. lia. }
+  Qed.
+
+
+  #[global] Instance anyR_observe_frac_valid ty :
+    TCSimpl (zero_sized_array ty) false -> CFracValid0 (anyR ty).
+  Proof.
+    rewrite anyR.unlock.
+    constructor =>q.
+    rewrite everywhereR_unfold.
+    revert q; induction ty; simpl; refine _.
+    { revert H.
+      simpl. rewrite /qual_norm/=.
+      case_bool_decide.
+      { inversion 1. }
+      { intros. iIntros "H".
+        have ->: (n = N.succ (n - 1))%N by lia.
+        rewrite replicateN_S. rewrite arr.arrayR_cons.
+        iDestruct "H" as "[? [H ?]]".
+        iDestruct (IHty with "H") as "$"; eauto. } }
+    { case_match; refine _.
+      case_match; refine _. }
+    { intros.
+      iIntros "H".
+      iDestruct (IHty with "H") as "%".
+      { by erewrite zero_sized_array_qual. }
+      { rewrite qualify_frac in H0.
+        eauto. } }
+  Qed.
+
+  #[global] Instance anyR_as_fractional ty : AsCFractional0 (anyR ty).
+  Proof. solve_as_cfrac. Qed.
+
+  Lemma anyR_disjoint (l : ptr) ty b1 b2 :
+    TCSimpl (zero_sized_array ty) false ->
+    l |-> anyR ty (cQp.mk b1 1) |-- l |-> anyR ty (cQp.mk b2 1) -* False.
+  Proof.
+    iIntros (?) "K L". iCombine "K L" as "P".
+    by iDestruct (observe [| _ ≤ 1 |]%Qp with "P") as %?.
+  Qed.
+
+  Lemma anyR_Tqualified t tq q : anyR (Tqualified tq t) q -|- anyR t (qualify tq q).
+  Proof. by rewrite anyR.unlock everywhereR_Tqualified. Qed.
+
+  (**
+  For value types and reference types, [anyR] coincides with
+  [tptstoR].
+  *)
+  Lemma tptstoR_anyR_val : ∀ t q v,
+      tptstoR t q v |-- anyR t q.
+  Proof.
+    induction t; simpl; try tauto;
+      try solve
+        [ intros; rewrite anyR.unlock everywhereR_unfold/primitiveR/=; eauto
+        | intros;
+          iIntros "H"; iDestruct (observe [| is_heap_type _ |] with "H") as "%H";
+          exfalso; revert H;
+          rewrite /is_heap_type /=; by rewrite andb_false_r ].
+    { (* pointers *)
+      iIntros (??) "H".
+      iDestruct (observe [| is_heap_type _ |] with "H") as "%H".
+      rewrite anyR.unlock everywhereR_unfold/primitiveR/=.
+      iExists v; iStopProof. f_equiv.
+      rewrite /is_heap_type in H.
+      case_bool_decide; auto. exfalso; done. }
+    { (* ref *)
+      iIntros (??) "H".
+      iDestruct (observe [| is_heap_type _ |] with "H") as "%H".
+      rewrite anyR.unlock everywhereR_unfold/primitiveR/=.
+      iExists v; iStopProof. f_equiv.
+      rewrite /is_heap_type in H.
+      case_bool_decide; auto. exfalso; done. }
+    { (* member_pointer *)
+      iIntros (??) "H".
+      iDestruct (observe [| is_heap_type _ |] with "H") as "%H".
+      rewrite anyR.unlock everywhereR_unfold/primitiveR/=.
+      iExists v; iStopProof. f_equiv.
+      rewrite /is_heap_type in H.
+      case_bool_decide; auto. exfalso; done. }
+    { (* qualified *)
+      intros.
+      intros;
+        iIntros "H"; iDestruct (observe [| is_heap_type _ |] with "H") as "%H".
+      exfalso; eauto using heap_type_not_qualified. }
+  Qed.
+
+  Lemma anyR_tptstoR_val : ∀ t q,
+      is_value_type t ->
+      anyR t q |-- Exists v, tptstoR (erase_qualifiers (decompose_type t).2) (qualify (decompose_type t).1 q) v.
+  Proof.
+    induction t; simpl; try tauto;
+      try solve [
+                    intros; rewrite anyR.unlock/everywhereR/=;
+          iIntros "X"; iDestruct "X" as (f) "X";
+            destruct f; [ iDestruct "X" as "[]" | simpl; eauto ]
+
+          | intros; rewrite anyR.unlock/everywhereR/=;
+          iSplit;
+          [ iIntros "X"; iDestruct "X" as (f) "X";
+            destruct f; [ iDestruct "X" as "[]" | simpl; eauto ]
+          | iIntros "X"; iExists 1; simpl; auto ] ].
+    { intros. rewrite anyR_Tqualified IHt; first last.
+      { rewrite -is_value_type_drop_qualifiers in H.
+        simpl in H.
+        rewrite -is_value_type_drop_qualifiers; done. }
+      f_equiv. intro.
+      rewrite -erase_qualifiers_decompose_type.
+      Opaque decompose_type.
+      rewrite qual_norm_decompose_type. simpl.
+      rewrite -erase_qualifiers_decompose_type/=.
+      f_equiv.
+      rewrite decompose_type_qual/=.
+      by rewrite qualify_merge_tq merge_tq_comm.
+      Transparent decompose_type. }
+  Qed.
+  Lemma anyR_tptstoR_ref t q :
+      anyR (Tref t) q -|- Exists v, tptstoR (Tref (erase_qualifiers t)) q v.
+  Proof.
+    (* todo: should be derived for [typeR] *)
+    intros.
+    rewrite anyR.unlock.
+    rewrite everywhereR_unfold/=.
+    rewrite /primitiveR/=. eauto.
+  Qed.
+  Lemma anyR_tptstoR_rv_ref t q :
+      anyR (Trv_ref t) q -|- Exists v, tptstoR (Tref (erase_qualifiers t)) q v.
+  Proof.
+    intros.
+    rewrite anyR.unlock.
+    rewrite everywhereR_unfold/=.
+    rewrite /primitiveR/=. eauto.
+  Qed.
+
+  Lemma primR_anyR : ∀ t q v,
+      primR t q v |-- anyR t q.
+  Proof.
+    intros.
+    rewrite primR.unlock.
+    iIntros "(%&#HT&Hp)".
+    iDestruct (observe [| has_type_prop _ _ |] with "HT") as %Ht.
+    rewrite tptsto_fuzzyR.unlock.
+    iDestruct "Hp" as (?) "[% Hp]".
+    rewrite -tptstoR_anyR_val. eauto.
+  Qed.
+  Lemma uninitR_anyR : ∀ t q,
+      uninitR t q |-- anyR t q.
+  Proof.
+    intros.
+    rewrite uninitR.unlock.
+    rewrite -tptstoR_anyR_val. eauto.
+  Qed.
+
+
+  Lemma tptstoR_anyR_ref t q v :
+    tptstoR (Tref t) q v |-- anyR (Tref t) q.
+  Proof.
+    intros. rewrite anyR_tptstoR_ref.
+    iIntros "H"; iExists _.
+    iDestruct (observe [| is_heap_type _ |] with "H") as "%H".
+    rewrite /is_heap_type in H.
+    case_bool_decide; auto. rewrite H0. eauto. exfalso; done.
+  Qed.
+
+  Lemma anyR_tptsto_fuzzyR_val_2 t q v :
+    is_value_type t -> tptsto_fuzzyR t q v |-- anyR t q.
+  Proof.
+    intros. rewrite tptsto_fuzzyR.unlock. iIntros "(% & % & R)".
+    rewrite -tptstoR_anyR_val; eauto.
+  Qed.
+
+  #[global] Instance anyR_type_ptr_observe ty q :
+    TCSimpl match to_heap_type ty with
+            | Tarray _ _ => false
+            | _ => true
+            end true →
+    Observe (type_ptrR $ to_heap_type ty) (anyR ty q).
+  Proof.
+    intros; rewrite anyR.unlock.
+    rewrite everywhereR_unfold.
+    revert q; induction ty; simpl; refine _; simpl in *; try tauto.
+    { inversion H. }
+    { case_match; refine _.
+      case_match; refine _. }
+  Qed.
+
+  #[global]
+  Instance anyR_valid_observe {ty q} : Observe validR (anyR ty q).
+  Proof.
+    rewrite anyR.unlock /everywhereR.
+    iIntros "H"; iDestruct "H" as (?) "H". iStopProof.
+    apply everywhereR_f_valid.
+    rewrite /primitiveR. intros.
+    iIntros "H"; iDestruct "H" as (?) "H".
+    iStopProof.
+    case_match; try solve [ iIntros "X"; iDestruct (observe validR with "X") as "$" ].
+  Qed.
+
+  #[global] Instance anyR_nonnull_observe : ∀ {ty q},
+      TCSimpl (zero_sized_array ty) false ->
+      Observe nonnullR (anyR ty q).
+  Proof.
+    rewrite anyR.unlock /everywhereR. intros.
+    iIntros "H"; iDestruct "H" as (?) "H". iStopProof.
+    apply everywhereR_f_nonnull; eauto.
+    rewrite /primitiveR. intros.
+    iIntros "H"; iDestruct "H" as (?) "H".
+    iStopProof.
+    case_match; try solve [ iIntros "X"; iDestruct (observe nonnullR with "X") as "$" ].
+    inversion H as [H1]; rewrite H1. auto.
+  Qed.
+
+  (** decompose a struct into its constituent fields and base classes. *)
+  Lemma anyR_struct : forall cls st q,
+    glob_def σ cls = Some (Gstruct st) ->
+        anyR (Tnamed cls) q
+    -|- Reduce (struct_defR anyR cls st q).
+  Proof.
+    intros. rewrite {1}anyR.unlock everywhereR_unfold/=.
+    have->: types (genv_tu σ) !! cls = Some (Gstruct st) by done.
+    rewrite /struct_defR anyR.unlock.
+    iSplit; iIntros "($&$&$)".
+  Qed.
+
+  (** decompose a union into the classical disjunction of the alternatives
+   *)
+  Lemma anyR_union : forall (cls : globname) un q,
+    glob_def σ cls = Some (Gunion un) ->
+        anyR (Tnamed cls) q
+    -|- Reduce (union_defR anyR cls un q).
+  Proof.
+    intros. rewrite {1}anyR.unlock everywhereR_unfold/=.
+    have->: types (genv_tu σ) !! cls = Some (Gunion un) by done.
+    rewrite /union_defR anyR.unlock.
+    done.
+  Qed.
+
+  (** Proof requires the generalization of [anyR] to support aggregates (and arrays) *)
+  Lemma anyR_array_0 t q :
+    anyR (Tarray t 0) q -|- validR ** [| is_Some (size_of σ t) |].
+  Proof.
+    rewrite anyR.unlock everywhereR_unfold/=.
+    by rewrite replicateN_0 arr.arrayR_nil.
+  Qed.
+
+  Lemma anyR_array_succ t n q :
+    anyR (Tarray t (N.succ n)) q -|-
+    type_ptrR t ** anyR t q ** .[ t ! 1 ] |-> anyR (Tarray t n) q.
+  Proof.
+    rewrite anyR.unlock everywhereR_unfold/=.
+    rewrite replicateN_S arr.arrayR_cons !everywhereR_unfold.
+    f_equiv. f_equiv. simpl. done.
+  Qed.
+
+  (** decompose an array into individual components
+      note that one past the end of an array is a valid location, but
+      it doesn't store anything.
+
+      TODO this should move
+   *)
+  Lemma anyR_array' t n q :
+        anyR (Tarray t n) q
+    -|- arr.arrayR t (fun _ => anyR t q) (replicateN n ()).
+  Proof.
+    induction n using N.peano_ind;
+      rewrite (replicateN_0, replicateN_S) (arr.arrayR_nil, arr.arrayR_cons).  {
+      apply anyR_array_0.
+    }
+    by rewrite -IHn anyR_array_succ.
+  Qed.
+
+  (* Wrapper using [repeat] instead of [replicate] for compatibility. *)
+  Lemma anyR_array t n q :
+        anyR (Tarray t n) q
+    -|- arr.arrayR t (fun _ => anyR t q) (repeat () (N.to_nat n)).
+  Proof. by rewrite anyR_array' repeatN_replicateN. Qed.
+
+  Lemma _at_anyR_ptr_congP_transport : forall p p' ty q,
+    ptr_congP σ p p' ** type_ptr ty p' |-- p |-> anyR ty q -* p' |-> anyR ty q.
+  Proof. (* TODO: this is very interesting *) Admitted.
+
+End with_cpp.
+
+#[deprecated(since="20231127",note="use [tptstoR_anyR_val]")] Notation anyR_tptstoR_val_2 := tptstoR_anyR_val (only parsing).
