theories/lang/cpp/logic/heap_pred/null.v
@@ -1,0 +1,89 @@
+(*
+ * Copyright (c) 2023 BedRock Systems, Inc.
+ * This software is distributed under the terms of the BedRock Open-Source License.
+ * See the LICENSE-BedRock file in the repository root for details.
+ *)
+Require Import bedrock.lang.cpp.logic.heap_pred.prelude.
+Require Import bedrock.lang.cpp.logic.heap_pred.valid.
+
+#[local] Set Printing Coercions.
+Implicit Types (σ : genv) (p : ptr) (o : offset).
+
+mlock Definition nullR `{Σ : cpp_logic} : Rep :=
+  as_Rep (fun addr => [| addr = nullptr |]).
+#[global] Arguments nullR {_ _} : assert.
+
+mlock Definition nonnullR `{Σ : cpp_logic} : Rep :=
+  as_Rep (fun addr => [| addr <> nullptr |]).
+#[global] Arguments nonnullR {_ _} : assert.	(* mlock bug *)
+
+Section with_cpp.
+  Context `{Σ : cpp_logic, σ : genv}.
+
+  Lemma _at_nullR p :
+      _at p nullR -|- [| p = nullptr |].
+  Proof. by rewrite nullR.unlock _at_as_Rep. Qed.
+
+  #[global] Instance nullR_persistent : Persistent nullR.
+  Proof. rewrite nullR.unlock. apply _. Qed.
+  #[global] Instance nullR_affine : Affine nullR.
+  Proof. rewrite nullR.unlock. apply _. Qed.
+  #[global] Instance nullR_timeless : Timeless nullR.
+  Proof. rewrite nullR.unlock. apply _. Qed.
+  #[global] Instance nullR_fractional : Fractional (λ _, nullR).
+  Proof. apply _. Qed.
+  #[global] Instance nullR_as_fractional q : AsFractional nullR (λ _, nullR) q.
+  Proof. exact: Build_AsFractional. Qed.
+  #[global] Instance nullR_cfractional : CFractional (λ _, nullR).
+  Proof. apply _. Qed.
+  #[global] Instance nullR_as_cfractional q : AsCFractional nullR (λ _, nullR) q.
+  Proof. solve_as_cfrac. Qed.
+
+  Lemma _at_nonnullR p : _at p nonnullR -|- [| p <> nullptr |].
+  Proof. by rewrite nonnullR.unlock _at_as_Rep. Qed.
+
+  #[global] Instance nonnullR_persistent : Persistent nonnullR.
+  Proof. rewrite unlock. apply _. Qed.
+  #[global] Instance nonnullR_affine : Affine nonnullR.
+  Proof. rewrite unlock. apply _. Qed.
+  #[global] Instance nonnullR_timeless : Timeless nonnullR.
+  Proof. rewrite unlock. apply _. Qed.
+
+  #[global] Instance type_ptrR_observe_nonnull ty :
+    Observe nonnullR (type_ptrR ty).
+  Proof.
+    rewrite nonnullR.unlock type_ptrR_eq /type_ptrR_def.
+    exact: as_Rep_observe.
+  Qed.
+
+  Lemma null_nonnull (R : Rep) : nullR |-- nonnullR -* R.
+  Proof.
+    rewrite nullR.unlock nonnullR.unlock.
+    constructor=>p /=. rewrite monPred_at_wand/=.
+    by iIntros "->" (? <-%ptr_rel_elim) "%".
+  Qed.
+
+  Lemma null_validR : nullR |-- validR.
+  Proof.
+    rewrite nullR.unlock validR_eq /validR_def.
+    constructor => p /=. iIntros "->". iApply valid_ptr_nullptr.
+  Qed.
+
+  #[global]
+  Instance null_valid_observe : Observe validR nullR.
+  Proof. rewrite -null_validR. refine _. Qed.
+
+  Lemma has_type_nullptr p :
+    has_type (Vptr p) Tnullptr -|- p |-> nullR.
+  Proof. by rewrite has_type_nullptr' nullR.unlock _at_as_Rep. Qed.
+
+End with_cpp.
+
+#[deprecated(note="since 2022-04-07; use `nullR` instead")]
+Notation is_null := nullR (only parsing).
+#[deprecated(note="since 2022-04-07; use `nullR.unlock` instead")]
+Notation is_null_eq := nullR.unlock (only parsing).
+(*
+#[deprecated(note="since 2022-04-07; use `nullR_def` instead")]
+Notation is_null_def := nullR_def (only parsing).
+*)
