theories/lang/cpp/logic/heap_pred/prelude.v
@@ -1,0 +1,18 @@
+(*
+ * Copyright (c) 2023 BedRock Systems, Inc.
+ * This software is distributed under the terms of the BedRock Open-Source License.
+ * See the LICENSE-BedRock file in the repository root for details.
+ *)
+From elpi.apps Require Export locker.
+
+From iris.proofmode Require Export proofmode.
+From bedrock.lang.bi Require Export fractional.
+
+From bedrock.lang.cpp Require Export
+  bi.cfractional
+  semantics ast logic.pred logic.pred logic.path_pred.
+
+Export bedrock.lang.cpp.logic.pred.
+(* ^^ Should this be exported? this file is supposed to provide wrappers
+   so that clients do not work directly with [pred.v] *)
+Export bedrock.lang.cpp.algebra.cfrac.
