theories/lang/cpp/logic/heap_pred/prim.v
@@ -1,0 +1,233 @@
+(*
+ * Copyright (c) 2023 BedRock Systems, Inc.
+ * This software is distributed under the terms of the BedRock Open-Source License.
+ * See the LICENSE-BedRock file in the repository root for details.
+ *)
+Require Import bedrock.lang.cpp.logic.heap_pred.prelude.
+From bedrock.lang.cpp.logic.heap_pred Require Import simple valid null tptsto uninit.
+
+#[local] Set Printing Coercions.
+Implicit Types (σ : genv) (p : ptr) (o : offset).
+
+(**
+[primR ty q v]: the argument pointer points to an initialized value
+[v] of C++ type [ty].
+
+NOTE [ty] *must* be a primitive type.
+*)
+mlock Definition primR `{Σ : cpp_logic, σ : genv} (ty : type) (q : cQp.t) (v : val) : Rep :=
+  [| ~~ is_raw v |] **
+  (**
+  NOTE: Clients use [primR (erase_qualifiers ty)] but we do not bake
+  [erase_qualifiers] in to simplify our automation.
+
+  TODO: In light of [has_type_drop_qualifiers], there's no need for
+  [drop_qualifiers].
+  *)
+  pureR (has_type v (drop_qualifiers ty)) **
+  tptsto_fuzzyR ty q v.
+#[global] Arguments primR {_ _ _} _ _ _ : assert.	(* mlock bug *)
+
+(* TODO: documentation needed *)
+mlock Definition reference_toR `{Σ : cpp_logic, σ : genv} (ty : type) : Rep :=
+  as_Rep (reference_to ty).
+#[global] Arguments reference_toR {_ _ _} _ : assert.	(* mlock bug *)
+
+#[global] Instance reference_toR_knoweldge `{Σ : cpp_logic, resolve : genv}
+  : Knowledge1 reference_toR.
+Proof. rewrite reference_toR.unlock; intros. split; refine _. Qed.
+#[global] Instance reference_toR_timeless `{Σ : cpp_logic, resolve : genv}
+  : Timeless1 reference_toR.
+Proof. rewrite reference_toR.unlock; intros. refine _. Qed.
+
+
+Section with_cpp.
+  Context `{Σ : cpp_logic} {σ : genv}.
+
+  Lemma _at_reference_toR ty (p : ptr) :
+    p |-> reference_toR ty -|- reference_to ty p.
+  Proof. by rewrite reference_toR.unlock _at_as_Rep. Qed.
+
+  Lemma _at_primR (p : ptr) ty q v :
+    p |-> primR ty q v -|-
+      [| ~~ is_raw v |] **
+      has_type v (drop_qualifiers ty) **
+      p |-> tptsto_fuzzyR ty q v.
+  Proof.
+    by rewrite primR.unlock !_at_sep _at_only_provable _at_pureR.
+  Qed.
+
+  #[global] Instance: Params (@primR) 2 := {}.
+  #[global] Instance primR_proper :
+    Proper (genv_eq ==> (=) ==> (=) ==> (=) ==> (⊣⊢)) (@primR _ _).
+  Proof.
+    intros σ1 σ2 Hσ ??-> ??-> ??->.
+    rewrite primR.unlock. by setoid_rewrite Hσ.
+  Qed.
+  #[global] Instance primR_mono :
+    Proper (genv_leq ==> (=) ==> (=) ==> (=) ==> (⊢)) (@primR _ _).
+  Proof.
+    intros σ1 σ2 Hσ ??-> ??-> ??->.
+    rewrite primR.unlock. by setoid_rewrite Hσ.
+  Qed.
+
+  #[global] Instance primR_timeless ty q v
+    : Timeless (primR ty q v).
+  Proof. rewrite primR.unlock. apply _. Qed.
+
+  #[global] Instance primR_cfractional ty :
+    CFractional1 (primR ty).
+  Proof. rewrite primR.unlock. apply _. Qed.
+  #[global] Instance primR_as_cfractional ty :
+    AsCFractional1 (primR ty).
+  Proof. solve_as_cfrac. Qed.
+
+  #[global] Instance primR_observe_cfrac_valid ty :
+    CFracValid1 (primR ty).
+  Proof. rewrite primR.unlock. solve_cfrac_valid. Qed.
+
+  Section TEST.
+    Context (p : ptr).
+
+    Goal
+        p |-> primR Tint (cQp.m (1/2)) 0
+        |-- p |-> primR Tint (cQp.m (1/2)) 0 -* p |-> primR Tint (cQp.m 1) 0.
+    Proof.
+      iIntros "H1 H2".
+      iCombine "H1 H2" as "$".
+    Abort.
+
+    Goal
+        p |-> primR Tint (cQp.c 1) 0 |-- p |-> primR Tint (cQp.c (1/2)) 0 ** p |-> primR Tint (cQp.c (1/2)) 0.
+    Proof.
+      iIntros "H".
+      iDestruct "H" as "[H1 H2]".
+    Abort.
+
+    Goal p |-> primR Tint (cQp.c 1) 1 |-- True.
+    Proof.
+      iIntros "H".
+      iDestruct (observe [| 1 ≤ 1 |]%Qp with "H") as %? (* ; [] << FAILS *).
+    Abort.
+  End TEST.
+
+  #[global] Instance primR_observe_agree ty q1 q2 v1 v2 :
+    Observe2 [| v1 = v2 |] (primR ty q1 v1) (primR ty q2 v2).
+  Proof.
+    rewrite primR.unlock. iIntros "(% & _ & R1) (% & _ & R2)".
+    iDestruct (observe_2 [| val_related _ _ _ |] with "R1 R2") as %?.
+    eauto using val_related_not_raw.
+  Qed.
+
+  (* Typical [f] are [Vint], [Vn] etc; this gives agreement for [u64R] etc. *)
+  #[global] Instance primR_observe_agree_constr ty q1 q2 {A} f `{!Inj eq eq f} (v1 v2 : A) :
+    Observe2 [| v1 = v2 |]
+      (primR ty q1 (f v1))
+      (primR ty q2 (f v2)).
+  Proof. apply (observe2_inj f), _. Qed.
+
+  #[global] Instance primR_observe_has_type ty q v :
+    Observe (pureR (has_type v ty)) (primR ty q v).
+  Proof. rewrite primR.unlock has_type_drop_qualifiers. apply _. Qed.
+
+  #[global] Instance _at_primR_observe_has_type ty q v (p : ptr) :
+    Observe (has_type v ty) (p |-> primR ty q v).
+  Proof. apply: _at_observe_pureR. Qed.
+
+  #[global] Instance primR_observe_has_type_prop ty q v :
+    Observe [| has_type_prop v ty |] (primR ty q v).
+  Proof.
+    apply observe_at=>p. rewrite _at_only_provable -has_type_has_type_prop.
+    apply _.
+  Qed.
+
+  Lemma primR_has_type_prop ty q v :
+    primR ty q v |--
+    primR ty q v ** [| has_type_prop v ty |].
+  Proof. apply: observe_elim. Qed.
+
+  Lemma primR_tptsto_acc p ty q v :
+    p |-> primR ty q v |--
+      Exists v', [| val_related ty v v' |] ** tptsto ty q p v' **
+      (Forall p' q' v', [| val_related ty v v' |] -* tptsto ty q' p' v' -* p' |-> primR ty q' v).
+  Proof.
+    setoid_rewrite _at_primR. iIntros "(%Hraw & #T & R)".
+    iDestruct (tptsto_fuzzyR_tptsto_acc with "R") as "(%v' & %Hval & R & HR)".
+    iExists v'. iFrame (Hval Hraw) "R T". iFrame "HR".
+  Qed.
+
+  #[global] Instance _at_primR_reference_to p ty q v :
+    Observe (reference_to ty p) (p |-> primR ty q v) | 100.
+  Proof. rewrite _at_primR. refine _. Qed.
+
+
+  Lemma test:
+    forall σ ty v v',
+      v' = Vundef ->
+      val_related ty v v' ->
+      v = Vundef.
+  Proof.
+    intros * Hv' Hval_related.
+    induction Hval_related;
+      try (by inversion Hv'); auto.
+  Succeed Qed. Abort.
+
+  (** This seems odd, but it's relevant to the (former) proof that [anyR] is
+  fractional; currently unused. *)
+  Lemma primR_uninitR ty q1 q2 v :
+    primR ty q1 v |--
+    uninitR ty q2 -*
+    primR ty (q1 + q2) Vundef.
+  Proof.
+    rewrite primR.unlock uninitR_tptstoR. iIntros "(_ & #T & R1) R2".
+    iDestruct (observe_2 [| val_related _ _ _ |] with "R2 R1") as %->%val_related_Vundef.
+    iFrame "T". iDestruct (tptsto_fuzzyR_elim_l with "[$R1 $R2]") as "R".
+    by iDestruct (tptsto_fuzzyR_intro with "R") as "$".
+  Qed.
+
+  #[global]
+  Instance primR_type_ptr_observe ty q v : Observe (type_ptrR ty) (primR ty q v).
+  Proof. rewrite primR.unlock. apply _. Qed.
+
+  (** Observing [valid_ptr] *)
+  #[global]
+  Instance primR_valid_observe {ty q v} : Observe validR (primR ty q v).
+  Proof. rewrite -svalidR_validR -type_ptrR_svalidR; refine _. Qed.
+
+  #[global]
+  Instance observe_type_ptr_pointsto (p : ptr) ty (R : Rep) :
+    Observe (type_ptrR ty) R -> Observe (type_ptr ty p) (_at p R).
+  Proof. rewrite -_at_type_ptrR. apply _at_observe. Qed.
+
+  Lemma primR_tptsto_fuzzyR ty q v : primR ty q v |-- tptsto_fuzzyR ty q v.
+  Proof. rewrite primR.unlock. iIntros "(_ & _ & $)". Qed.
+
+  #[global]
+  Instance primR_nonnull_observe {ty q v} :
+    Observe nonnullR (primR ty q v).
+  Proof. rewrite primR.unlock. apply _. Qed.
+
+  (** ** [reference_to] *)
+  #[global] Instance reference_to_valid ty p : Observe (valid_ptr p) (reference_to ty p).
+  Proof. rewrite reference_to_elim. refine _. Qed.
+  #[global] Instance reference_to_aligned ty p : Observe [| aligned_ptr_ty ty p |] (reference_to ty p).
+  Proof. rewrite reference_to_elim. refine _. Qed.
+  #[global] Instance reference_to_aligned_ofR ty (p : ptr) : Observe (p |-> aligned_ofR ty) (reference_to ty p).
+  Proof. rewrite reference_to_elim aligned_ofR_aligned_ptr_ty. refine _. Qed.
+  #[global] Instance reference_to_not_null ty p : Observe [| p <> nullptr |] (reference_to ty p).
+  Proof. rewrite reference_to_elim. refine _. Qed.
+  #[global] Instance reference_to_strict_valid ty p :
+    TCEq (zero_sized_array ty) false ->
+    Observe (strict_valid_ptr p) (reference_to ty p).
+  Proof. rewrite reference_to_elim. move => ->. refine _. Qed.
+
+
+  #[global] Instance reference_to_aligned_observe p ty :
+    Observe (p |-> aligned_ofR ty) (reference_to ty p).
+  Proof. rewrite aligned_ofR_aligned_ptr_ty reference_to_elim; refine _. Qed.
+  #[global] Instance reference_to_valid_observe p ty :
+    Observe (p |-> validR) (reference_to ty p).
+  Proof. rewrite _at_validR reference_to_elim; refine _. Qed.
+
+
+End with_cpp.
