theories/lang/cpp/logic/heap_pred/simple.v
@@ -1,0 +1,116 @@
+(*
+ * Copyright (c) 2023 BedRock Systems, Inc.
+ * This software is distributed under the terms of the BedRock Open-Source License.
+ * See the LICENSE-BedRock file in the repository root for details.
+ *)
+Require Import bedrock.lang.cpp.logic.heap_pred.prelude.
+From bedrock.lang.cpp.logic.heap_pred Require Import valid.
+
+#[local] Set Printing Coercions.
+Implicit Types (σ : genv) (p : ptr) (o : offset).
+
+(** ** Object derivations
+    The path from the object to its complete object.
+  *)
+mlock
+Definition derivationR `{Σ : cpp_logic} {σ : genv} (cls : globname) (mdc : list globname)
+  (q : cQp.t) : Rep :=
+    as_Rep (mdc_path cls mdc q).
+#[global] Arguments derivationR {_ Σ σ} _ _ _.
+
+mlock
+Definition alignedR `{Σ : cpp_logic} (al : N) : Rep :=
+  as_Rep (λ p, [| aligned_ptr al p |]).
+#[global] Arguments alignedR {_ Σ} _.
+
+(* [Rep] version of (to be deprecated) [aligned_ptr_ty] *)
+mlock
+Definition aligned_ofR `{Σ : cpp_logic} {σ} (ty : type) : Rep :=
+  ∃ align : N, [| align_of ty = Some align |] ** alignedR align.
+#[global] Arguments aligned_ofR {_ Σ σ} _.
+
+Section with_cpp.
+  Context `{Σ : cpp_logic} {σ : genv}.
+
+  (** ** [alignedR] *)
+  #[global] Instance alignedR_persistent {al} : Persistent (alignedR al).
+  Proof. rewrite alignedR.unlock. apply _. Qed.
+  #[global] Instance alignedR_affine {al} : Affine (alignedR al).
+  Proof. rewrite alignedR.unlock. apply _. Qed.
+  #[global] Instance alignedR_timeless {al} : Timeless (alignedR al).
+  Proof. rewrite alignedR.unlock. apply _. Qed.
+
+  #[global] Instance alignedR_divide_mono :
+    Proper (flip N.divide ==> bi_entails) alignedR.
+  Proof.
+    intros m n ?.
+    rewrite alignedR.unlock. constructor=>p/=. iIntros "!%".
+    exact: aligned_ptr_divide_weaken.
+  Qed.
+
+  #[global] Instance alignedR_divide_flip_mono :
+    Proper (N.divide ==> flip bi_entails) alignedR.
+  Proof. solve_proper. Qed.
+
+  Lemma alignedR_divide_weaken m n :
+    (n | m)%N ->
+    alignedR m ⊢ alignedR n.
+  Proof. by move->. Qed.
+
+  (* To use sparingly: we're deprecating [aligned_ptr] *)
+  Lemma _at_alignedR (p : ptr) n :
+    p |-> alignedR n -|- [| aligned_ptr n p |].
+  Proof. by rewrite alignedR.unlock _at_as_Rep. Qed.
+
+  #[global] Instance aligned_ofR_persistent {ty} : Persistent (aligned_ofR ty).
+  Proof. rewrite aligned_ofR.unlock. apply _. Qed.
+  #[global] Instance aligned_ofR_affine {ty} : Affine (aligned_ofR ty).
+  Proof. rewrite aligned_ofR.unlock. apply _. Qed.
+  #[global] Instance aligned_ofR_timeless {ty} : Timeless (aligned_ofR ty).
+  Proof. rewrite aligned_ofR.unlock. apply _. Qed.
+
+  Lemma aligned_ofR_aligned_ptr_ty p ty :
+    p |-> aligned_ofR ty -|- [| aligned_ptr_ty ty p |].
+  Proof.
+    rewrite aligned_ofR.unlock alignedR.unlock /aligned_ptr_ty _at_exists only_provable_exist.
+    f_equiv => n. rewrite _at_sep _at_as_Rep _at_only_provable.
+    by iIntros "!%".
+  Qed.
+
+  Lemma type_ptrR_aligned_ofR ty :
+    type_ptrR ty |-- aligned_ofR ty.
+  Proof.
+    apply Rep_entails_at => p.
+    by rewrite _at_type_ptrR type_ptr_aligned_pure aligned_ofR_aligned_ptr_ty.
+  Qed.
+
+  Lemma type_ptr_aligned_ofR p ty :
+    type_ptr ty p |-- p |-> aligned_ofR ty.
+  Proof. by rewrite -type_ptrR_aligned_ofR _at_type_ptrR. Qed.
+
+  (** ** [derivationR] *)
+  #[global] Instance derivationR_timeless cls mdc q : Timeless (derivationR cls mdc q).
+  Proof. rewrite derivationR.unlock. refine _. Qed.
+  #[global] Instance derivationR_cfractional cls mdc : CFractional (derivationR cls mdc).
+  Proof. rewrite derivationR.unlock. refine _. Qed.
+  #[global] Instance derivationR_as_frac cls mdc :
+    AsCFractional0 (derivationR cls mdc).
+  Proof. solve_as_cfrac. Qed.
+
+  #[global] Instance derivationR_strict_valid cls mdc q : Observe svalidR (derivationR cls mdc q).
+  Proof.
+    red. eapply Rep_entails_at. intros.
+    rewrite derivationR.unlock _at_as_Rep _at_pers svalidR_eq _at_as_Rep.
+    apply mdc_path_strict_valid.
+  Qed.
+  #[global] Instance mdc_path_not_null p cls path q
+    : Observe [| p <> nullptr |] (p |-> derivationR cls path q).
+  Proof.
+    red.
+    iIntros "X".
+    destruct (decide (p = nullptr)); eauto.
+    iDestruct (observe (p |-> svalidR) with "X") as "#SV".
+    subst; rewrite _at_svalidR not_strictly_valid_ptr_nullptr.
+    iDestruct "SV" as "[]".
+  Qed.
+End with_cpp.
